% make a template 
\documentclass[12pt]{article}
\usepackage{amsmath}
\title{HW4}
\author{Dev Goyal}
\date{April 2023}

\begin{document}
\maketitle

\section*{Problem 1}

\noindent \textbf{Task 1}: \newline
\begin {equation}
\begin{split}
    \varphi (r,s) = (\forall r',s'. \ (r*(90*s + 20*(1-s)) + (1-r)*(30*s + 60*(1-s)) \\ \geq r'*(90*s + 20*(1-s)) + (1-r')*(30*s + 60*(1-s))) \\ 
    \land (s*(r*10 + 70 * (1-r)) + (1-s)*(r*80 + (1-r)*40 \\ \geq s'*(r*10 + 70 * (1-r)) + (1-s')*(r*80 + (1-r)*40)))\\ \land (r \geq 0) \land (s \geq 0) \land (r \leq 1) \land (s \leq 1) \land (r' \geq 0) \land (s' \geq 0) \land (r' \leq 1) \land (s' \leq 1))
\end{split}
\end {equation}

\noindent \textbf{Task 2}: \newline

the link for the Z3 code is: https://github.com/devg24/CS474/tree/main/HW4

The code outputs sat and gives the equilibrium as r = 0.3 and s = 0.5.

\noindent \textbf{Task 3}: \newline

Let r,s be mixed strategies for each player and let F,B denote two outcomes. This is to say that player 1 chooses f with probability r and b with probability 1-r and player 2 chooses f with probability s and b with probability 1-s. let $p_{ff}$ denote the payoff for player 1 when both players choose f and $p_{fb}$ denote the payoff for player 1 when player 1 chooses f and player 2 chooses b. Let $p_{bf}$ denote the payoff for player 1 when player 1 chooses b and player 2 chooses f and $p_{bb}$ denote the payoff for player 1 when both players choose b. Let $q_{ff}$ denote the payoff for player 2 when both players choose f and $q_{fb}$ denote the payoff for player 2 when player 1 chooses f and player 2 chooses b. Let $q_{bf}$ denote the payoff for player 2 when player 1 chooses b and player 2 chooses f and $q_{bb}$ denote the payoff for player 2 when both players choose b.:

\begin {equation}
\begin{split}
    \psi \equiv \exists r,s . \forall p_{ff}, p_{fb}, p_{bf}, p_{bb}, q_{ff}, q_{fb}, q_{bf}, q_{bb}, r', s' \\ 
    (r*(p_{ff}*s + p_{fb}*(1-s)) + (1-r)*(p_{bf}*s + p_{bb}*(1-s)) \\ \geq r'*(p_{ff}*s + p_{fb}*(1-s)) + (1-r')*(p_{bf}*s + p_{bb}*(1-s))) \\ 
    \land (s*(r*q_{ff} + q_{fb} * (1-r)) + (1-s)*(r*q_{bf} + (1-r)*q_{bb} \\ \geq s'*(r*q_{ff} + q_{fb} * (1-r)) + (1-s')*(r*q_{bf} + (1-r)*q_{bb})))\\ \land (r \geq 0) \land (s \geq 0) \land (r \leq 1) \land (s \leq 1) \land (r' \geq 0) \land (s' \geq 0) \land (r' \leq 1) \land (s' \leq 1)
\end{split}
\end {equation}

the link for the Z3 code is: https://github.com/devg24/CS474/tree/main/HW4


\section*{Problem 2}

The set of terms T is:

\{a, f(a), g(a), f(g(a)), f(f(a)), f(f(f(a)))\}

the set of equalities E is:

\{ (f(f(f(a))), f(a)), (f(a),g(a)), (f(g(a)), a)\}

the set of inequalities I is:

\{(a,f(a))\}

We start with the equivalence relation:

\{ \{a\}, \{f(a)\}, \{g(a)\}, \{f(g(a))\}, \{f(f(a))\}, \{f(f(f(a)))\} \}

since f(a) and g(a) are equal, we can merge the sets:

\{ \{a\}, \{f(a), g(a)\}, \{f(g(a))\}, \{f(f(a))\}, \{f(f(f(a)))\} \}

since f(g(a)) and a are equal, we can merge the sets:

\{ \{a, f(g(a))\}, \{f(a), g(a)\}, \{f(f(a))\}, \{f(f(f(a)))\} \}

since f(f(f(a))) and f(a) are equal, we can merge the sets:

\{ \{a, f(g(a))\}, \{f(a), g(a), f(f(f(a)))\}, \{f(f(a))\} \}

since f(a) and g(a) are in the same equivalence class, we have to merge the equivalence class of f(f(a)) and f(g(a)):

\{ \{a, f(g(a)), f(f(a))\}, \{f(a), g(a), f(f(f(a)))\} \}

since f(f(a)) and g(a) are in T so we have to merge f(f(f(a))) and f(g(a)) which yields the following equivalence relation:

\{ \{a, f(g(a)), f(f(a)), f(f(f(a))), f(a), g(a)\} \}

since a and f(a)  are in I so this means that the model is unsatisfiable.


\section*{Problem 3}
\noindent Task 1:

The formula is :

\begin {equation}
\varphi : \forall e'. ((\forall x. (f(x,e') = x \land f(e',x) = x) \implies (e' = e)))
\end{equation}

following the steps in the book by bringing the formula to a prenex form and then negating it we get:

\begin {equation}
\neg \varphi: \exists e'. \forall x (f(x,e') = x \land f(e',x) = x \land \neg (e' = e))
\end{equation}

now skolemizing by replacing the quantified variable e' with a new constant c we get:

\begin {equation}
\forall x. (f(x,c) = x \land f(c,x) = x \land \neg (c = e))
\end {equation}

The four universal formulae we get are now :
\begin{enumerate}
    \item $\forall x,y,z. f(f(x,y),z) = f(x,f(y,z))$
   
    \item $\forall x. f(x,e) = x \land f(e,x) = x$

    \item $\forall x. f(x , g(x)) = e \land f(g(x),x) = e$

    \item $\forall x. (f(x,c) = x \land f(c,x) = x \land \neg (c = e))$
\end{enumerate}

instantiating terms of depth 0 we get the following formulae:
\begin{enumerate}
    \item $f(f(e,e),e) = f(e,f(e,e))$
    \item $f(f(c,e),e) = f(c,f(e,e))$
    \item $f(f(e,c),e) = f(e,f(c,e))$
    \item $f(f(c,c),e) = f(c,f(c,e))$
    \item $f(f(e,e),c) = f(e,f(e,c))$
    \item $f(f(c,e),c) = f(c,f(e,c))$
    \item $f(f(e,c),c) = f(e,f(c,c))$
    \item $f(f(c,c),c) = f(c,f(c,c))$
    \item $f(e,e) = e \land f(e,e) = e$
    \item $f(c,e) = c \land f(e,c) = c$
    \item $f(e , g(e)) = e \land f(g(e),e) = e$
    \item $f(c , g(c)) = e \land f(g(c),c) = e$
    \item $(f(e,c) = e \land f(c,e) = e \land \neg (c = e))$
    \item $(f(c,c) = c \land f(c,c) = c \land \neg (c = e))$
\end{enumerate}

Putting this in smt2 form tields unsat which is the expected result.

link: \textbf{https://github.com/devg24/CS474/tree/main/HW4}

\noindent Task 2:

The formula is :

\begin {equation}
\varphi : \forall x, y. (f(x,y) = e \land f(y,x) = e) \implies (y = g(x))
\end {equation}

where g(x) is the inverse function.

negating the above and skolemizing using two new constant symbol c and d gives:

$$(f(c,d) = e \land f(d,c) = e) \land \neg(d = g(c))$$

The four universal formulae we get are now :

\begin{enumerate}
    \item $\forall x,y,z. f(f(x,y),z) = f(x,f(y,z))$
    \item $\forall x. f(x,e) = x \land f(e,x) = x$
    \item $\forall x. f(x , g(x)) = e \land f(g(x),x) = e$
    \item $(f(c,d) = e \land f(d,c) = e) \land \neg(d = g(c))$
\end{enumerate}

instantiating terms of depth 0 we get the following formulae:

\begin{enumerate}
    \item Substituting e for x, e for y, and e for z:
    $f(f(e,e),e) = f(e,f(e,e))$
    
    \item Substituting e for x, e for y, and c for z:
    $f(f(e,e),c) = f(e,f(e,c))$
    
    \item Substituting e for x, e for y, and d for z:
    $f(f(e,e),d) = f(e,f(e,d))$
    
    \item Substituting e for x, c for y, and e for z:
    $f(f(e,c),e) = f(e,f(c,e))$
    
    \item Substituting e for x, c for y, and c for z:
    $f(f(e,c),c) = f(e,f(c,c))$
    
    \item Substituting e for x, c for y, and d for z:
    $f(f(e,c),d) = f(e,f(c,d))$
    
    \item Substituting e for x, d for y, and e for z:
    $f(f(e,d),e) = f(e,f(d,e))$
    
    \item Substituting e for x, d for y, and c for z:
    $f(f(e,d),c) = f(e,f(d,c))$
    
    \item Substituting e for x, d for y, and d for z:
    $f(f(e,d),d) = f(e,f(d,d))$
    
    \item Substituting c for x, e for y, and e for z:
    $f(f(c,e),e) = f(c,f(e,e))$
    
    \item Substituting c for x, e for y, and c for z:
    $f(f(c,e),c) = f(c,f(e,c))$
    
    \item Substituting c for x, e for y, and d for z:
    $f(f(c,e),d) = f(c,f(e,d))$
    
    \item Substituting c for x, c for y, and e for z:
    $f(f(c,c),e) = f(c,f(c,e))$
    
    \item Substituting c for x, c for y, and c for z:
    $f(f(c,c),c) = f(c,f(c,c))$
    
    \item Substituting c for x, c for y, and d for z:
    $f(f(c,c),d) = f(c,f(c,d))$
    
    \item Substituting c for x, d for y, and e for z:
    $f(f(c,d),e) = f(c,f(d,e))$
    
    \item Substituting c for x, d for y, and c for z:
    $f(f(c,d),c) = f(c,f(d,c))$
    
    \item Substituting c for x, d for y, and d for z:
    $f(f(c,d),d) = f(c,f(d,d))$
    
    \item Substituting d for x, e for y, and e for z:
    $f(f(d,e),e) = f(d,f(e,e))$
    
    \item Substituting d for x, e for y, and c for z:
    $f(f(d,e),c) = f(d,f(e,c))$
    
    \item Substituting d for x, e for y, and d for z:
    $f(f(d,e),d) = f(d,f(e,d))$
    
    \item Substituting d for x, c for y, and e for z:
    $f(f(d,c),e) = f(d,f(c,e))$
    
    \item Substituting d for x, c for y, and c for z:
    $f(f(d,c),c) = f(d,f(c,c))$
    
    \item Substituting d for x, c for y, and d for z:
    $f(f(d,c),d) = f(d,f(c,d))$
    
    \item Substituting d for x, d for y, and e for z:
    $f(f(d,d),e) = f(d,f(d,e))$

    \item Substituting d for x, d for y, and c for z:
    $f(f(d,d),c) = f(d,f(d,c))$

    \item Substituting d for x, d for y, and d for z:
    $f(f(d,d),d) = f(d,f(d,d))$

    \item Substituting e for x:
    $f(e,e) = e \land f(e,e) = e$
    
    \item Substituting c for x:
    $f(c,e) = c \land f(e,c) = c$
    
    \item Substituting d for x:
    $f(d,e) = d \land f(e,d) = d$
    
    \item Substituting e for x:
    $f(e, g(e)) = e \land f(g(e),e) = e$

    \item Substituting c for x:
    $f(c, g(c)) = e \land f(g(c),c) = e$

    \item Substituting d for x:
    $f(d, g(d)) = e \land f(g(d),d) = e$

    \item $(f(c,d) = e \land f(d,c) = e) \land \neg(d = g(c))$
    
\end{enumerate}

Putting this in smt2 form tields unsat which is the expected result.

link: \textbf{https://github.com/devg24/CS474/tree/main/HW4}



\end{document}



