\documentclass{article}
\usepackage[utf8]{inputenc}
\usepackage{hyperref}
\usepackage{amsmath}

\title{HW1}
\author{Dev Goyal }
\date{February 2023}

\begin{document}

\maketitle

\section{Problem 1}

We're required to prove ($p \land (p \rightarrow q) \rightarrow q$) using resolution.

We will prove this by showing that the resolution of ($p \land (p \rightarrow q)) \land (\neg q$) is unsatisfiable.

We will now convert the expression to CNF.

\begin{itemize}
    \item replace $p \rightarrow q $ with $\neg p \lor q$
    \item the expression is now $(p \land \neg p \lor q) \land \neg q$
\end{itemize}
we can now apply resolution to the expression. We see that RHS contains q and LHS contains $\neg q$ so we can apply resolution to get an empty clause. Hence the expression is unsatisfiable.
and thus the original expression is valid.
\end{document}